Finalise proof for DSC.

src/dafny/smart/DepositSmart.dfy
@@ -26,6 +26,8 @@ include "./trees/Trees.dfy"
 include "./MerkleTrees.dfy"
 
 include "./intdiffalgo/IndexBasedAlgorithm.dfy"
+include "./intdiffalgo/CommuteProof.dfy"
+
 
 module DepositSmart {
 
@@ -43,407 +45,171 @@ module DepositSmart {
     import opened GenericComputation
 
     import opened IndexBasedAlgorithm
-    
+    import opened CommuteProof
+
     /**
      *  The functional version of the deposit smart contract.
      */
-    class Deposit<T> {
+    class Deposit {
 
         //  State Variables.
 
         /** The default value for the leaves. */
-        const d : T 
+        const d : int 
 
         /** The attribute function to synthesise. */
-        const f : (T, T) -> T
-
+        const f : (int, int) -> int
+    
         /** The height of the tree. */
         const TREE_HEIGHT : nat
 
         /** The values on the left siblings of the path to leaf of index k. */
-        var branch : seq<T>
+        var branch : seq<int>
 
         /** The value sof the right siblings of path to leaf at index k. */
-        const zero_h : seq<T>
+        const zero_h : seq<int>
 
         /** The number of values added to the list. Also the index of the next available leaf. */
         var count : nat 
 
         //  Ghost variables used for the correctness proof.
 
-        /** The number of values added to the tree. */
-        // ghost var count : nat 
+        /** The list of values added so far. */
+        ghost var values : seq<int> 
 
         /** The (Merkle) tree that corresponds to the list of values added so far. */
-        ghost var t : Tree<T>
+        ghost var t : Tree<int>
 
-        /** The value of the root of the tree. */
-        // ghost var r : T
-
-        /** The list of values added so far. */
-        ghost var values : seq<T> 
-
-        /** Path to index of next available leaf. */
+        /** Path to index of next available leaf at index |values|. */
         ghost var p : seq<bit>
-
-        /** The values on the left siblings on p. */
-        // ghost var left : seq<T>
 
         /** Property to maintain. */
         predicate Valid()
             reads this
         {
-            //  Height and sequences sizes
+            //  Height and sequences sizes.
             1 <= TREE_HEIGHT ==  height(t) == |branch| == |zero_h| == |p|
-            //  tree is not full
-            && count < power2(TREE_HEIGHT)
-
-            && |values| == count <= power2(TREE_HEIGHT) == |leavesIn(t)|
-
-            //  t is the Merkle tree for the valuea added so far. 
+            //  Maximum number of values stored in the tree bounded.
+            && count < power2(TREE_HEIGHT) == |leavesIn(t)|
+            //  count is the number of values added so far.
+            && |values| == count
+            //  t is the Merkle tree for values. 
             && isMerkle(t, values, f, d) && hasLeavesIndexedFrom(t, 0)
-
+            //  zero_h is constant and equal to default values for each level of t.
             && zero_h == zeroes(f, d, TREE_HEIGHT - 1)
-            && (forall i :: 0 <= i < |zero_h| ==> 
-                    zero_h[i] == defaultValue(f, d, height(t) - 1 - i)
-            )
-            //  The right siblings of the current path are all zeroes
+            //  Left and right siblings of `p` are given by branch and zero_h.
             && (forall i :: 0 <= i < |p| ==> 
-                    siblingValueAt(p, t, i + 1) == 
-                        if p[i] == 0 then
-                             zero_h[i]
-                        else 
-                            branch[i]
+                siblingValueAt(p, t, i + 1) == 
+                    if p[i] == 0 then zero_h[i] else branch[i]
             )
-
-            // && (r == t.v)
-            //  Path is to current next free leaf.
-            // && bitListToNat(p) == count
+            //  `p` is the path to the next available slot at index `count`.
             && p == natToBitList(count, TREE_HEIGHT)
-            // && nodeAt(p, t) == leavesIn(t)[count]
-            // && nodeAt(p, t).v == lastVal
-
-            //  Branch has values of left siblings of current path
-            // && (forall i :: 0 <= i < |branch| && p[i] == 1 ==> 
-            //         siblingValueAt(p, t, i + 1) == branch[i])
-
-            // && (forall i :: 0 <= i < |left| && p[i] == 1 ==> 
-            //         siblingValueAt(p, t, i + 1) == left[i])
         }
 
         /**
          *  Initialise the system, tree of size >= 1.
          */
-        constructor(h: nat, l : seq<T>, default : T, fun : (T, T) -> T) 
+        constructor(h: nat, l : seq<int>, f1 : (int, int) -> int, default : int) 
             requires h >= 1
-            requires |l| == h && forall i :: 0 <= i < |l| ==> l[i] == default
+            requires |l| == h && forall i :: 0 <= i < |l| ==> l[i] == 0
             ensures Valid()
         {
             //  State variables
-
-            TREE_HEIGHT, count, d, f := h, 0, default, fun;
-            branch, zero_h := l, zeroes(fun, default, h - 1);
+            TREE_HEIGHT, count, f, d := h, 0, f1, default;
+            branch, zero_h := l, zeroes(f1, default, h - 1);
 
             //  Ghost variables
-
-            //  The initial tree is the Merkle tree for brancn (or l).
-            t := buildMerkle([], h, fun, default);
-            //  The values that have been added is initially empty.
-            values := [];
-            //  possibly left could be left uninitialised
-            // left := l;
-            //  Path to the first available leaf at index 0.
-            p := natToBitList2(0, h);
+            t, values, p := buildMerkle([], h, f1, default), [],  natToBitList(0, h);
+            
+            //  Proof that right siblings of p are zero_h.
             bitToNatToBitsIsIdentity(0, h);
             valueIsZeroImpliesAllZeroes(natToBitList2(0, h));
-            leafAtPathIsIntValueOfPath(natToBitList2(0, h), buildMerkle([], h, fun, default), 0, 0);
-
-            rightSiblingsOfLastPathAreDefault(natToBitList2(0, h), buildMerkle([], h, fun, default), 0, fun, 0, default);
-            //  Initially r is value of f for all leaves equal to default.
-            // r := defaultValue(fun, default, h);
-            //  Use lemma to prove that r == t.v
-            allLeavesDefaultImplyRootNodeDefault(buildMerkle([], h, fun, default), fun, default);
+            leafAtPathIsIntValueOfPath(natToBitList2(0, h), buildMerkle([], h, f1, default), 0, 0);
+            rightSiblingsOfLastPathAreDefault(natToBitList2(0, h), buildMerkle([], h, f1, default), 0, f1, 0, default);
         }
 
-        
-        method dep(v : T) 
+        /**
+         *  Deposit.
+         *  
+         *  @param  v   The new deposit amount.
+         */
+        method deposit(v : int) 
             requires Valid()
             requires count < power2(TREE_HEIGHT) - 1         
-
-            ensures 1 <= TREE_HEIGHT ==  height(t) == |branch| == |zero_h| == |p|
-            ensures values == old(values) + [v]
-            ensures 1 <= |values| <= power2(height(t))
-            ensures count == old(count) + 1
-            ensures exists i :: 0 <= i < |old(p)| && old(p)[i] == 0
-            ensures p == nextPath(old(p))
-
-            ensures isMerkle(t, values, f, d) && hasLeavesIndexedFrom(t, 0)
-            ensures p == natToBitList(count, TREE_HEIGHT)
-            ensures count < power2(TREE_HEIGHT)
-            ensures |values| == count <= power2(TREE_HEIGHT) == |leavesIn(t)|
-
-            ensures zero_h == zeroes(f, d, TREE_HEIGHT - 1)
-            ensures (forall i :: 0 <= i < |p| ==> 
-                    siblingValueAt(p, t, i + 1) == 
-                        if p[i] == 0 then
-                             zero_h[i]
-                        else 
-                            branch[i])
-           
-            // ensures Valid()
-
+            ensures Valid()
             modifies this 
         {
-            t := buildMerkle(values + [v], TREE_HEIGHT, f, d);
+            ghost var tt :=  buildMerkle(values + [v], TREE_HEIGHT, f, d);
+            assert(p == natToBitList(|values|, TREE_HEIGHT));
 
-            nextPathSameSiblingsInNextList(TREE_HEIGHT, values, v, old(t), t, f, d, p);
-            assert(
-                reveal_siblingValueAt();
-                forall i :: 0 <= i < |p|  ==>
-                    siblingValueAt(p, t, i + 1) == siblingValueAt(p, old(t), i + 1)
-            );
-
-            assert(
-                reveal_siblingValueAt();
-                forall i :: 0 <= i < |p| ==> 
-                    siblingValueAt(p, t, i + 1) == 
-                    siblingValueAt(p, old(t), i + 1) == 
+            //  Siblings of p in t are same as siblings on p in old(t)
+            forall (i : nat | 0 <= i < |p|)
+                ensures siblingValueAt(p, tt, i + 1) == 
+                     siblingValueAt(p, old(t), i + 1) ==
                         if p[i] == 0 then
                              zero_h[i]
                         else 
                             branch[i]
-            );
-
-            values := values + [v];
-
-            bitToNatToBitsIsIdentity(count, TREE_HEIGHT);
-            leafAtPathIsIntValueOfPath(p, t, count, 0);
+            {
+                 reveal_siblingValueAt();
+                 nextPathSameSiblingsInNextList(
+                    TREE_HEIGHT, values, v, old(t), 
+                    tt, 
+                    f, d, p);
+            }
             
-            computeLeftSiblingOnNextPathFromLeftRightIsCorrectInATree(p, t, branch, zero_h, f, v, count);
-
-            assert(
-                forall i :: 0 <= i < |p| && nextPath(p)[i] == 1 ==> 
-                computeLeftSiblingOnNextPathFromLeftRight(p, branch, zero_h, f, v)[i] == siblingAt(take(nextPath(p), i + 1),t ).v
-            );
-
-            branch := computeLeftSiblingsOnNextpathWithIndex(TREE_HEIGHT, count, branch, zero_h, f, v);
-
             bitToNatToBitsIsIdentity(count, TREE_HEIGHT);
             pathToNoLasthasZero(p);
             assert(exists i :: 0 <= i < |p| && p[i] == 0);
 
-            p := nextPath(p);
-
-            assert(count == old(count));
-            count := count + 1;
-            assert count == old(count) + 1;
+             forall ( i : nat | 0 <= i < |nextPath(p)| && nextPath(p)[i] == 1)
+                ensures computeLeftSiblingOnNextPathFromLeftRight(p, branch, zero_h, f, v)[i]
+                    ==
+                    siblingValueAt(nextPath(p), tt, i + 1) 
+            {
+                computeLeftSiblingOnNextPathFromLeftRightIsCorrectInAMerkleTree(
+                    p, values, v, tt, branch, zero_h, f, d
+                );
+            }
 
             pathToSucc(old(p), old(count), TREE_HEIGHT);
+            assert(nextPath(p) == natToBitList(old(count) + 1, TREE_HEIGHT));
 
+            //  Compute new branch (this is the algorithm).
+            branch := computeLeftSiblingsOnNextpathWithIndex(TREE_HEIGHT, count, branch, zero_h, f, v);
+            count := count + 1;
+
+            //  Update ghost vars
+            values := values + [v];
+            p := nextPath(p);
+            t := buildMerkle(values, TREE_HEIGHT, f, d);
+            
+            pathToLastInMerkleTreeHasZeroRightSiblings(p, values, t, f, d);
+            assert(
+                forall i :: 0 <= i < |p| && p[i] == 0 ==> 
+                    siblingValueAt(p, t, i + 1) == zero_h[i]
+            );
             assert(
                 forall i :: 0 <= i < |p| && p[i] == 1 ==> 
-                    branch[i] == siblingAt(take(p, i + 1),t ).v
+                    siblingValueAt(p, t, i + 1) == branch[i]
             );
+        }   
 
-            
-            assume(p == natToBitList(|values| - 1, TREE_HEIGHT));
-            assume(height(t) == TREE_HEIGHT);
-
-            // pathToLastInMerkleTreeHasZeroRightSiblings(p, values, t, f, d);
-            // assert(
-            //     // reveal_siblingValueAt();
-            //     forall i :: 0 <= i < |p| && p[i] == 0 ==> 
-            //         // siblingValueAt(p, t, i + 1) 
-            //         // siblingAt(take(p, i + 1),t ).v ==
-            //         zeroes(f, d, height(t) - 1)[i] 
-            //         == zero_h[i]
-            // );
-            forall ( i : nat | 0 <= i < |p| && p[i] == 0) 
-                // ensures siblingAt(take(p, i + 1),t ).v 
-                ensures siblingValueAt(p, t, i + 1) ==  zeroes(f, d, height(t) - 1)[i] 
-                // == zero_h[i]
-            {
-                //  reveal_siblingValueAt();
-                pathToLastInMerkleTreeHasZeroRightSiblings(p, values, t, f, d);
-            }
-        }
-        
         /**
-         *  Deposit a value i.e update the state.
+         *  This method should always return the root value of the tree.
+         *
+         *  @returns    The root value of the Merkle Tree for values.
          */
-        // method deposit(v : T) 
-        //     requires Valid()
-        //     requires count < power2(TREE_HEIGHT) - 1 
-            
-        //     ensures 1 <= TREE_HEIGHT ==  height(t) == |branch| == |zero_h| == |left| == |p|
-        //     ensures count < power2(TREE_HEIGHT) 
-        //     ensures |values| == count < power2(TREE_HEIGHT) == |leavesIn(t)|
-        //     ensures isMerkle(t, values, f, d)
-
-        //     ensures p == natToBitList(old(count) + 1, TREE_HEIGHT)
-        //     ensures count == old(count) + 1
-        //     ensures p == natToBitList(count, TREE_HEIGHT)
-
-        //     // ensures (forall i :: 0 <= i < |p| && p[i] == 1 ==> 
-        //     //         siblingValueAt(p, t, i + 1) == branch[i]
-                        
-        //     // ensures nodeAt(p, t) == leavesIn(t)[count]
-
-        //     //  left siblings post condition
-
-
-        //     modifies this 
-        // {
-        //     t := buildMerkle(values + [v], TREE_HEIGHT, f, d);
-        //     assert(hasLeavesIndexedFrom(t, 0));
-        //     assert(isCompleteTree(t));
-        //     bitToNatToBitsIsIdentity(old(count), TREE_HEIGHT) ;
-        //     bitToNatToBitsIsIdentity(count, TREE_HEIGHT) ;
-        //     assert( bitListToNat(old(p)) == old(count));
-        //     assert( bitListToNat(p) == count);
-        //     leafAtPathIsIntValueOfPath(p, t, count, 0);
-        //     leafAtPathIsIntValueOfPath(old(p), t, old(count), 0);
-        //     assert(nodeAt(old(p), t) == leavesIn(t)[old(count)]);
-        //     assert(nodeAt(p, t) == leavesIn(t)[count]);
-
-
-        //     nextPathSameSiblingsInNextList(TREE_HEIGHT, values, v, old(t), t, f, d, p);
-        //     assert(
-        //         reveal_siblingValueAt();
-        //         forall i :: 0 <= i < |p|  ==>
-        //             siblingValueAt(p, t, i + 1) == siblingValueAt(p, old(t), i + 1)
-        //     );
-
-        //     computeLeftSiblingOnNextPathFromLeftRightIsCorrectInATree(old(p), t, branch, zero_h, f, v, old(count));
-
-        //     // computeLeftSiblingOnNextPathFromLeftRightIsCorrectInATree(p, t, branch, zero_h, f, v, count);
-
-        //     // assert(
-        //     //     forall i :: 0 <= i < |old(p)| && nextPath(old(p))[i] == 1 ==> 
-        //     //     computeLeftSiblingOnNextPathFromLeftRight(old(p), branch, zero_h, f, v)[i] == siblingAt(take(nextPath(old(p)), i + 1),t ).v
-        //     // );
-
-        //     //  prove properties on left siblings.
-
-        //     values := values + [v];
-
-        //     //  before computing nextPath(p), prove bitListToNat(p) < power2(|p|) - 1
-        //     bitToNatToBitsIsIdentity(old(count), TREE_HEIGHT) ;
-        //     pathToNoLasthasZero(old(p));
-        //     assert(bitListToNat(old(p)) < power2(|old(p)|) - 1);
-            
-        //     p :=  nextPath(p);
-            
-        //     ghost var x := computeLeftSiblingsOnNextpathWithIndex(TREE_HEIGHT, count, old(branch), zero_h, f, v);
-        //     //  Compute left siblings on next path to (count + 1)-th leaf. 
-        //     branch := computeLeftSiblingsOnNextpathWithIndex(TREE_HEIGHT, count, branch, zero_h, f, v);
-        //     assert(branch == x
-        //         // computeLeftSiblingsOnNextpathWithIndex(TREE_HEIGHT, count, old(branch), zero_h, f, v)
-        //         == computeLeftSiblingOnNextPathFromLeftRight(natToBitList(count, TREE_HEIGHT), old(branch), zero_h, f, v)
-        //     );
-        //     //
-            
-
-        //     count := count + 1;
-        //     assert(count == old(count) + 1);
-        //     assert(old(count) < power2(TREE_HEIGHT) - 1);
-        //     assert(count ==  old(count) + 1 < power2(TREE_HEIGHT) - 1 + 1);
-        //     assert(p ==  nextPath(old(p)));
-        //     pathToSucc(old(p), old(count), TREE_HEIGHT);
-        //     assert(p == natToBitList(count, TREE_HEIGHT));
-            
-        //     //  branch is left siblings on path to count
-        //     // assert();
-        //     // assert (forall i :: 0 <= i < |p| && p[i] == 1 ==> 
-        //     //         siblingValueAt(p, t, i + 1) == branch[i]);
-        // }
-
-
-        method get_deposit_root() returns (h_root: T) 
+        method get_deposit_root() returns ( r : int) 
             requires Valid()
-            requires count < power2(TREE_HEIGHT) - 1 
-
-            // ensures count == 0 ==> h_root == t.v 
+            ensures Valid()
+            /** The result is the root value of the tree.  */
+            ensures r == t.v 
         {
-            //  Show that d == nodeAt(p, t).v
-            // calc == {
-            //     nodeAt(p, t).v;
-            //     leavesIn(t)[natToBitList2(count, h)].v;
+            r := computeRootLeftRightUpWithIndex(TREE_HEIGHT, count, branch, zero_h, f, d);
 
-            // }
-            // assume(d == nodeAt(p, t).v);
-            // assert(bitListToNat(p) == count);
-            // bitToNatToBitsIsIdentity(count, TREE_HEIGHT);
-            // assert(p == natToBitList(count, TREE_HEIGHT));
-
-            // reveal_siblingValueAt();
-            // computeRootLeftRightUpIsCorrectForTree(p, t, branch, zero_h, f, d);
- 
-            //  Compute the root using the left siblings on next path (branch) and default value d.
-            h_root := computeRootLeftRightUpWithIndex(TREE_HEIGHT, count, branch, zero_h, f, d);
-            // assert(
-            //     computeRootLeftRightUpWithIndex(TREE_HEIGHT, count, branch, zero_h, f, d)
-            //     ==
-            //     computeRootLeftRightUp(natToBitList2(count, TREE_HEIGHT), branch, zero_h, f, d)
-            //     ==
-            //     computeRootLeftRightUp(p, branch, zero_h, f, d)
-
-            // );
-            // assert(t.v == computeRootLeftRightUp(p, branch, zero_h, f, d));
+            //  The proof of post condition follows easily from:
+            computeRootUsingDefaultIsCorrectInAMerkleTree(p, values, t, branch, zero_h, f, d);
         }
-
-        
-
-        /**
-         *  Deposit a value i.e update the state.
-         */
-        // method deposit2(value : T) 
-        //     requires Valid()
-        //     requires count < power2(TREE_HEIGHT) - 1 
-
-        //     modifies this 
-        // {
-            //  Update ghost variables that simulate what is happening on the Merkle tree.
-            //  Add value to tree 
-            // values := values + [value];
-            // assert(|values| == count + 1 < power2(TREE_HEIGHT));
-            // t := buildMerkle(values, TREE_HEIGHT, f, d);
-            // assert(height(t) == TREE_HEIGHT);
-            // assert(isMerkle(t, values, f, d));
-
-            // nextPathSameSiblingsInNextList(TREE_HEIGHT, old(values), value, old(t), t, f, d, p, nextPath(p));
-            // r := computeRootLeftRightUpWithIndex(TREE_HEIGHT, count + 1, branch, zero_h, f, value);
-            // computeWithIndexFromZeroIsCorrect(TREE_HEIGHT, count, branch, zero_h, f, value);
-            // computeRootLeftRightIsCorrectForTree(natToBitList(count, TREE_HEIGHT), t, branch, zero_h, f, value);
-            // assert(r == t.v);            
-
-            // //  Compute nextPath
-            // //  We have to show p (path to count-th leaf, has a zero
-            // assert(bitListToNat(p) == count < power2(TREE_HEIGHT) - 1 == power2(|p|) - 1);
-            // pathToNoLasthasZero(p);
-            // p := nextPath(p);
-            // //  p is path to (count + 1)-th leaf
-            // nextPathIffSucc(old(p), p);
-            // assert(bitListToNat(p) == bitListToNat(old(p)) + 1 == count + 1);
-            // leafAtPathIsIntValueOfPath(p, t, count + 1 , 0);
-            // assert(nodeAt(p, t) == leavesIn(t)[count + 1]);
-
-            // computeLeftSiblingOnNextPathFromLeftRightIsCorrectInATree(natToBitList(count + 1, TREE_HEIGHT), t, branch, zero_h, f, value, count);
-
-           
-            //  Depsoit contract algorithm
-            //  Compute left siblings on next path to (count + 1_th leaf. 
-            // branch := computeLeftSiblingsOnNextpathWithIndex(TREE_HEIGHT, count, branch, zero_h, f, value);
-            // count := count + 1;
-
-            // assert();
-
-            //  branch is the value of siblings on next path.
-            // assert(branch == computeLeftSiblingOnNextPathFromLeftRight(natToBitList(count, TREE_HEIGHT), left, zero_h, f, value));
-            
-            // computeLeftSiblingOnNextPathFromLeftRight();
-        // }
-
     }
-
 }
